Finish `fresh_key_package`

fstar/new/MLS.Crypto.Builtins.fst
@@ -174,6 +174,11 @@ let sign_signature_length cs =
   | Ed_25519 -> 64
   | P_256 -> 0 //TODO
 
+let sign_gen_keypair cs rand =
+  match cs.signature with
+  | Ed_25519 ->
+      return (rand, Ed25519.secret_to_public rand)
+  | P_256 -> internal_failure "sign_gen_keypair: P_256 not implemented"
 
 let sign_sign cs sk msg rand =
   match cs.signature with
